Work on state machines proofs towards verifying list combinator

core/Core.v
@@ -126,8 +126,6 @@ Module ByteListReader : READER.
     reflexivity.
   Qed.
 
-  Definition state_machine (S A : Type) := byte -> S -> fold_state S A.
-
   Fixpoint fold {S A}
            (f : state_machine S A) (s : S) (l : list byte) :=
     match l with
@@ -174,12 +172,13 @@ Module ByteListReader : READER.
   Lemma fold_pair_inr : forall S1 A S2 B
                                (a : state_machine S1 A) (b : state_machine S2 B)
                                x bytes s,
-      (fold (pair a b) (inr (x, s))) bytes =
-      match fold b s bytes with
+      unwrap (fold (pair a b) (inr (x, s))) bytes =
+      match unwrap (fold b s) bytes with
       | Some (y, l) => Some ((x, y), l)
       | Nones => None
       end.
   Proof.
+    unfold unwrap.
     intros until bytes.
     induction bytes.
     - reflexivity.
@@ -192,12 +191,13 @@ Module ByteListReader : READER.
   Lemma fold_pair_inl : forall S1 A S2 B
                                (a : state_machine S1 A) (b : state_machine S2 B)
                                bytes s1 s2,
-      (fold (pair a b) (inl (s1, s2))) bytes =
-      match fold a s1 bytes with
-      | Some (x, l) => fold (pair a b) (inr (x, s2)) l
+      unwrap (fold (pair a b) (inl (s1, s2))) bytes =
+      match unwrap (fold a s1) bytes with
+      | Some (x, l) => unwrap (fold (pair a b) (inr (x, s2))) l
       | None => None
       end.
   Proof.
+    unfold unwrap.
     intros until bytes.
     induction bytes.
     - reflexivity.
@@ -230,12 +230,13 @@ Module ByteListReader : READER.
                                   (a : state_machine S1 A)
                                   (b : state_machine S2 B)
                                   bytes f s,
-      (fold (sequence a b) (inl (s, f))) bytes =
-      match fold a s bytes with
+      unwrap (fold (sequence a b) (inl (s, f))) bytes =
+      match unwrap (fold a s) bytes with
       | Some (x, bytes) => fold (sequence a b) (inr (f x)) bytes
       | None => None
       end.
   Proof.
+    unfold unwrap.
     induction bytes.
     - reflexivity.
     - intros.
@@ -248,8 +249,9 @@ Module ByteListReader : READER.
                                   (a : state_machine S1 A)
                                   (b : state_machine S2 B)
                                   bytes s,
-      fold (sequence a b) (inr s) bytes = fold b s bytes.
+      unwrap (fold (sequence a b) (inr s)) bytes = unwrap (fold b s) bytes.
   Proof.
+    unfold unwrap.
     induction bytes; simpl; intros.
     - reflexivity.
     - destruct b; auto.
@@ -265,11 +267,14 @@ Module ByteListReader : READER.
                   end.
   
   Definition countdown {S A}
-             (f : S -> A)
+             (f : S -> option A)
              (a : state_machine S A) : state_machine (S * nat) A :=
     fun byte s =>
       match s with
-      | (s, O) => Done (f s)
+      | (s, O) => match f s with
+                  | Some v => Done v
+                  | None => Error
+                  end
       | (s, S n) => match a byte s with
                     | Done a => Done a
                     | More s => More (s, n)
@@ -277,7 +282,7 @@ Module ByteListReader : READER.
                     end
       end.
 
-  Definition list {S A} (a : state_machine S A) (init : S) := countdown snd (list_acc a init).
+  Definition list {S A} (a : state_machine S A) (init : S) := countdown (fun x => Some (snd x)) (list_acc a init).
 
   Lemma ret_unwrap : forall {A} (x: A) bytes, unwrap (ret x) bytes = Some (x, bytes).
   Proof. reflexivity. Qed.
